floyd/proofauto.v
@@ -2,6 +2,7 @@ From compcert Require Export common.AST cfrontend.Ctypes cfrontend.Clight.
 Export Cop.
 Require Export VST.floyd.base2.
 Require Export VST.floyd.sublist.
+Require Export VST.floyd.sublist2.
 Require Export VST.floyd.client_lemmas.
 Require Export VST.floyd.go_lower.
 Require Export VST.floyd.closed_lemmas.
