floyd/sublist2.v
@@ -1,0 +1,40 @@
+Require Import VST.floyd.base2.
+Require Import VST.floyd.val_lemmas.
+Require Import VST.floyd.sublist.
+
+Instance Inhabitant_val : Inhabitant val := Vundef.
+Instance Inhabitant_int: Inhabitant int := Int.zero.
+Instance Inhabitant_byte: Inhabitant byte := Byte.zero.
+Instance Inhabitant_int64: Inhabitant Int64.int := Int64.zero.
+Instance Inhabitant_ptrofs: Inhabitant Ptrofs.int := Ptrofs.zero.
+Instance Inhabitant_float : Inhabitant float := Float.zero.
+Instance Inhabitant_float32 : Inhabitant float32 := Float32.zero.
+
+Definition Vbyte (c: Byte.int) : val :=
+  Vint (Int.repr (Byte.signed c)).
+
+Lemma Znth_map_Vbyte: forall (i : Z) (l : list byte),
+  0 <= i < Zlength l -> Znth i (map Vbyte l)  = Vbyte (Znth i l).
+Proof.
+  intros i l.
+  apply Znth_map.
+Qed.
+Hint Rewrite Znth_map_Vbyte using list_solve : norm entailer_rewrite.
+
+Lemma is_int_Vbyte: forall c, is_int I8 Signed (Vbyte c).
+Proof.
+intros. simpl. normalize. rewrite Int.signed_repr by rep_omega. rep_omega.
+Qed.
+Hint Resolve is_int_Vbyte.
+
+Ltac fold_Vbyte :=
+ repeat match goal with |- context [Vint (Int.repr (Byte.signed ?c))] =>
+      fold (Vbyte c)
+end.
+
+Hint Rewrite 
+   (@Znth_map val _) (@Znth_map int _) (@Znth_map byte _)
+   (@Znth_map int64 _) (@Znth_map ptrofs _) (@Znth_map float _)
+   (@Znth_map float32 _)
+    using (auto; rewrite ?Zlength_map in *; omega) : sublist entailer_rewrite.
+
